concurrency/sync_preds.v
@@ -28,10 +28,10 @@ Require Import veric.semax_ext.
 Require Import veric.semax_ext_oracle.
 Require Import veric.res_predicates.
 Require Import veric.mem_lessdef.
+Require Import veric.coqlib4.
 Require Import sepcomp.semantics.
 Require Import sepcomp.step_lemmas.
 Require Import sepcomp.event_semantics.
-Require Import concurrency.coqlib5.
 Require Import concurrency.age_to.
 Require Import concurrency.semax_conc.
 Require Import concurrency.juicy_machine.
